src/iinductive.v
@@ -7,144 +7,58 @@ Require Import index wf IFunctor ISPFunctor.
 
 Section INDUCTIVE.
 
-  Variable I O : Type.
-  Variable F : O -> (I + O -> Type) -> Type.
+  Variable O : Type.
+  Variable F : O -> (O -> Type) -> Type.
 
   Context `{H : forall c, SPFunctor (F c)}.
-  Variable X : (iType I).
-
-  Definition X_ (T : O -> Type) : I + O -> Type :=
-    fun io : I + O => match io with
-                      | inl i => X i
-                      | inr o1 => T o1
-                      end.
-
-  Goal True. Proof. constructor. Qed.
-
-  Definition X_fun (T1 T2 : O -> Type) (f : forall o, T1 o -> T2 o) io :
-    X_ T1 io -> X_ T2 io :=
-    match io as io' return (X_ T1 io' -> X_ T2 io') with
-    | inl i => (fun x' => x')
-    | inr o => (fun x' => f o x')
-    end.
+  Variable X : (iType O).
 
   Inductive Mu : O -> Type :=
-  | Con' o : sigT (fun (s : S) =>
-                    ((forall (i : I), (@P _ _ (H o) s (inl i)) -> X i) *
-                     (forall (o1 : O), (@P _ _ (H o) s (inr o1)) -> Mu o1))%type)
-            -> Mu o.
+  | Con' o : Container (@P _ _ (H o)) Mu -> Mu o.
 
-  Definition Des' o (m : Mu o) : sigT (fun (s : S) =>
-                    ((forall (i : I), (@P _ _ (H o) s (inl i)) -> X i) *
-                     (forall (o1 : O), (@P _ _ (H o) s (inr o1)) -> Mu o1))%type) :=
+  Definition Con o (fx : F o Mu) : Mu o := Con' o (NT _ fx).
+
+  Definition Des' o (m : Mu o) : Container (@P _ _ (H o)) Mu :=
     match m with
     | Con' o s => s end.
 
-
-  (* I wanna define Mu as below *)
-  Fail Inductive Mu' : O -> Type :=
-  | Con'' o : sigT (fun (s : S) =>
-                     (forall (io : I + O), (@P _ _ (H o) s io) -> 
-                                           match io with
-                                           | inl i => X i
-                                           | inr o1 => Mu' o1
-                                           end)) -> Mu' o.
-   (* but this definition can't pass the coq's strict positivity checker *)
-
-  Definition Con o (fx : F o (X_ Mu)) : Mu o :=
-    match (NT _ fx) with
-    | existT _ s f => Con' o (existT _ s
-                                     ((fun i (p : P s (inl i)) => f (inl i) p),
-                                      (fun o1 (p : P s (inr o1)) => f (inr o1) p))) end.
-
-  Definition Des o (m : Mu o) : F o (X_ Mu) :=
-    match m with
-    | Con' _ (existT _ s (f1, f2)) =>
-      NTinv _
-            (existT (fun s' => forall i, P s' i -> (X_ Mu) i) s
-                    (fun (io : I + O) (p : P s io) =>
-                       match io as io' return (P s io' -> (X_ Mu) io') with
-                       | inl i => fun p' : P s (inl i) => f1 i p'
-                       | inr o1 => fun p' : P s (inr o1) => f2 o1 p'
-                       end p)) end.
-
-  Goal True.
-    auto.
-  Qed.
+  Definition Des o (m : Mu o) : F o Mu := NTinv _ (Des' m).
 
   Lemma eta_expand2 : forall o (x : Mu o), Con (Des x) = x.
   Proof.
-    intros. unfold Des, Con. destruct x as [o m].
-    destruct m as [s [f1 f2]]. rewrite BIJECTION2.
-    f_equal.
+    intros. unfold Des, Con. rewrite BIJECTION2.
+    destruct x. reflexivity.
   Qed.
 
-  Lemma eta_expand1 : forall o (x : F o (X_ Mu)), Des (Con x) = x.
+  Lemma eta_expand1 : forall o (x : F o Mu), Des (Con x) = x.
   Proof.
     intros. unfold Des, Con.
-    destruct (NT _ x) eqn : EQ.
-    rewrite <- BIJECTION1. f_equal. rewrite EQ. f_equal.
-    extensionality io. extensionality p.
-    destruct io; reflexivity.
+    rewrite <- BIJECTION1.
+    destruct (NT Mu x). reflexivity.
   Qed.
-  (* if we define Mu as Mu', extensionality isn't necessary *)
-
-(*
-  Inductive ord : forall o1, Mu o1 -> forall o2, Mu o2 -> Prop :=
-  | _ord (o1 o2 : O) (s : S) (p : P s (inr o1)) f1 f2 :
-      ord (f2 o1 p) (Con' o2 (existT _ s (f1, f2))).
-*)
 
   Definition ord : forall o1, Mu o1 -> forall o2, Mu o2 -> Prop :=
-    fun o1 m1 o2 m2 =>
-      exists (p : P (projT1 (Des' m2)) (inr o1)),
-        (m1 = (snd (projT2 (Des' m2))) o1 p).
+   fun o1 m1 o2 m2 => mem (Des' m2) m1.
 
   Lemma ord_wf : iwell_founded ord.
   Proof.
     unfold iwell_founded. fix 2.
     intros o2 m2. constructor.
-    intros o1 m1 ORD. destruct ORD as [p H1].
-    rewrite H1. apply ord_wf.
+    intros o1 m1 ORD. destruct ORD.
+    rewrite <- H0. apply ord_wf.
   Qed.
 
   Definition ord_c := iclos_transn1 ord.
 
-(*
-  Lemma ORD_LEMMA o1 o2 (x1 : Mu o1) (x2 : Mu o2) :
-    ord x1 x2 ->
-    exists s (f1 : forall i : I, P s (inl i) -> X i)
-             (f2 : forall x : O, P s (inr x) -> Mu x) (p : P s (inr o1)), x1 = f2 o1 p /\ x2 = Con' o2 (existT _ s (f1, f2)).
+  Lemma ord_correct : forall o1 (m : Mu o1) o2 (fx : F o2 Mu),
+      @mem O (F o2) _ Mu fx o1 m <-> ord m (Con fx).
   Proof.
-    intro.
-    destruct H0. exists s. exists f1. exists f2. eauto.
-  Qed.
-*)
-
-  Lemma Con'_INJ : forall o x y, Con' o x = Con' o y -> x = y.
-  Proof.
-    intros. apply f_equal with (f := @Des' o) in H0.
-    simpl in H0. apply H0.
-  Qed.
-
-  Lemma ord_correct : forall o1 (m : Mu o1) o2 (fx : F o2 (X_ Mu)),
-      @mem (I + O) (F o2) _ (X_ Mu) fx (inr o1) m <-> ord m (Con fx).
-  Proof.
-    intros; split; [intro MEM | intro ORD].
-    - apply MEM_COMMUTE in MEM. simpl in MEM.
-      unfold Con. destruct (NT _ fx) eqn : EQ.
-      apply CONTAINER_MEM in MEM. destruct MEM.
-      rewrite <- H0. unfold ord. exists x1; reflexivity.
-    - apply MEM_COMMUTE. unfold Con in ORD.
-      destruct (NT _ fx). simpl in *. unfold ord in ORD. simpl in *.
-      destruct ORD. apply CONTAINER_MEM.
-      exists x1. symmetry. apply H0.
+    intros. rewrite MEM_COMMUTE. reflexivity.
   Qed.
 
   Lemma ord_c_wf : iwell_founded ord_c.
   Proof.
-    apply wf_iclos_trans.
-    apply ord_wf.
+    apply wf_iclos_trans. apply ord_wf.
   Qed.
 
   Lemma ord_transitive o1 o2 o3 (x : Mu o1) (y : Mu o2) (z : Mu o3) :
@@ -152,24 +66,6 @@ Section INDUCTIVE.
   Proof.
     apply iclos_transn1_transitive.
   Qed.
-
-  Definition Des_ord o (m : Mu o) : F o (X_ (sigI (fun i x => @ord_c i x _ m))).
-    eapply (map _ (tag _ (Des m))).
-    Unshelve.
- destruct i. simpl in *.
-
-    - apply (@projI1 _ _ (@mem (I + O) (F o) Fn (X_ Mu) (Des m))).
-    - 
-
-      intro. 
-
-      eapply existI.
-      
-      
-      set (itn1_step _ ord (eq_ind _ _ ((proj1 (iff_and ((ord_correct (projI1 X0)) o (Des m)))) (projI2 X0)) _ (eta_expand2 m))). 
-      apply i.
-
-  Defined.
 
   Definition rec (P : forall o, Mu o -> Type)
              (FIX : forall o1 (m1 : Mu o1), 
@@ -189,20 +85,32 @@ Section INDUCTIVE.
     forall o, Mu o -> T :=
     rec_simpl1 _ FIX.
 
-  Definition prim_rec1 (P : forall (o : O), Type)
-             (FIX : forall o, F o (X_ P) -> P o) :
-    forall o, Mu o -> P o :=
-    rec_simpl1 P
-               (fun (o1 : O) (m1 : Mu o1) (f : forall (o2 : O) (m2 : Mu o2), ord_c m2 m1 -> P o2) =>
-                  FIX o1 (map (X_fun (sigI (fun (i : O) (x : Mu i) => ord_c x m1)) P
-                                     (fun (o : O) (X0 : sigI (fun (i : O) (x : Mu i)
-                                                              => ord_c x m1) o) =>
-                                        f o (projI1 X0) (projI2 X0))) (Des_ord m1))).
+  Lemma rec_red (P : forall o, Mu o -> Type)
+        (FIX : forall o1 (m1 : Mu o1), 
+            (forall o2 (m2 : Mu o2), ord_c m2 m1 -> P o2 m2) -> P o1 m1)
+        o (fx : F o  Mu) :
+    rec _ FIX (Con fx) = FIX _ (Con fx) (fun _ fy _ => rec _ FIX fy).
+  Proof.
+    apply iFix_eq.
+  Qed.
 
-  Definition prim_rec2 T
-             (FIX : forall o, F o (X_ (fun _ => T)) -> T) :
-    forall o, Mu o -> T :=
-    prim_rec1 FIX.
+  Lemma rec_simpl1_red (P : forall o, Type)
+        (FIX : forall o1 (m1 : Mu o1), 
+            (forall o2 (m2 : Mu o2), ord_c m2 m1 -> P o2) -> P o1) 
+        o (fx : F o Mu) :
+    rec_simpl1 _ FIX (Con fx) = FIX _ (Con fx) (fun _ fy _ => rec_simpl1 _ FIX fy).
+  Proof.
+    apply (rec_red _ FIX fx).
+  Qed.
+
+  Lemma rec_simpl2_red T
+        (FIX : forall o1 (m1 : Mu o1), 
+            (forall o2 (m2 : Mu o2), ord_c m2 m1 -> T) -> T)
+        o (fx : F o Mu) :
+    rec_simpl2 FIX (Con fx) = FIX _ (Con fx) (fun _ fy _ => rec_simpl2 FIX fy).
+  Proof.
+    apply (rec_simpl1_red _ FIX fx).
+  Qed.
 
   Definition induction_principle (P : forall o, Mu o -> Prop)
              (FIX : forall o1 (m1 : Mu o1), 
@@ -221,67 +129,170 @@ Section INDUCTIVE.
   Qed.
 
   Definition mem_induction_principle (P : forall o, Mu o -> Prop)
-             (FIX : forall o1 (fx : F o1 (X_ Mu)), 
-                 (forall o2 (m : Mu o2), @mem (I + O) (F o1) _ (X_ Mu) fx (inr o2) m
-                                         -> P _ m) -> P _ (Con fx)) :
+             (FIX : forall o1 (fx : F o1 Mu), 
+                 (forall o2 (m : Mu o2), mem fx m -> P _ m) -> P _ (Con fx)) :
     forall o (m : Mu o), P o m.
   Proof.
     apply induction_principle.
-    intros.
-    revert H0. destruct (eta_expand2 m1).
-    intros.
-    apply FIX.
-    intros.
-    apply H0, ord_correct, H1.
+    intros o1 m1. destruct (eta_expand2 m1).
+    intros. apply FIX.
+    intros. apply H0, ord_correct, H1.
   Qed.
 
-  Lemma rec_red (P : forall o, Mu o -> Type)
-        (FIX : forall o1 (m1 : Mu o1), 
-            (forall o2 (m2 : Mu o2), ord_c m2 m1 -> P o2 m2) -> P o1 m1)
-        o (fx : F o (X_ Mu)) :
-    rec _ FIX (Con fx) = FIX _ (Con fx) (fun _ fy _ => rec _ FIX fy).
+  Lemma ord_lemma o (m : Mu o)
+    : forall (i : O) (x : Mu i), mem (Des m) x -> ord_c x m.
   Proof.
-    apply iFix_eq.
+    intros i x MEM.
+    rewrite <- eta_expand2. apply itn1_step, ord_correct, MEM.
   Qed.
 
-  Lemma rec_simpl1_red (P : forall o, Type)
-        (FIX : forall o1 (m1 : Mu o1), 
-            (forall o2 (m2 : Mu o2), ord_c m2 m1 -> P o2) -> P o1) 
-        o (fx : F o (X_ Mu)) :
-    rec_simpl1 _ FIX (Con fx) = FIX _ (Con fx) (fun _ fy _ => rec_simpl1 _ FIX fy).
+  Definition Des_ord o (m : Mu o) : F o (sigI (fun i x => @ord_c i x _ m)) :=
+    @map _ (F o) _ _ _ (sigImply _ (ord_lemma m)) (tag _ (Des m)).
+
+  Lemma Des_ord_correct o (fx : F o Mu)
+    : map (@projI1 _ _ _) (Des_ord (Con fx)) = fx.
   Proof.
-    apply (rec_red _ FIX fx).
+    unfold Des_ord. rewrite MAP_COMPOSE.
+    simpl. rewrite TAG. apply eta_expand1.
   Qed.
 
-  Lemma rec_simpl2_red T
-        (FIX : forall o1 (m1 : Mu o1), 
-            (forall o2 (m2 : Mu o2), ord_c m2 m1 -> T) -> T)
-        o (fx : F o (X_ Mu)) :
-    rec_simpl2 FIX (Con fx) = FIX _ (Con fx) (fun _ fy _ => rec_simpl2 FIX fy).
-  Proof.
-    apply (rec_simpl1_red _ FIX fx).
-  Qed.
+  Definition prim_rec1 (P : forall (o : O), Type)
+             (FIX : forall o, F o P -> P o) :=
+    rec_simpl1 P (fun o1 m1 f => FIX _ (map (fun o fx => f _ (projI1 fx) (projI2 fx))
+                                            (Des_ord m1))).
 
   Lemma prim_rec1_red (P : forall (o : O), Type)
-        (FIX : forall o, F o (X_ P) -> P o) o (fx : F o (X_ Mu)) :
-    prim_rec1 FIX (Con fx) = FIX _ (map (X_fun _ _ (prim_rec1 FIX)) fx).
+        (FIX : forall o, F o P -> P o) o (fx : F o Mu) :
+    prim_rec1 FIX (Con fx) = FIX o (map (prim_rec1 FIX) fx).
   Proof.
     unfold prim_rec1.
     rewrite rec_simpl1_red.
-    unfold X_fun. simpl in *. f_equal. unfold Des_ord.
-    rewrite MAP_COMPOSE. simpl in *. 
-    
-    
+    pattern fx at 5.
+    rewrite <- (Des_ord_correct fx).
+    rewrite MAP_COMPOSE. reflexivity.
+  Qed.    
 
-
-    
-  Admitted.
+  Definition prim_rec2 T
+             (FIX : forall o, F o (fun _ => T) -> T) :
+    forall o, Mu o -> T :=
+    prim_rec1 FIX.
   
-  Lemma prim_rec2_red T (FIX : forall o, F o (X_ (fun _ => T)) -> T)
-        o (fx : F o (X_ Mu)) :
-    prim_rec2 FIX (Con fx) = FIX _ (map (X_fun _ _ (prim_rec2 FIX)) fx).
+  Lemma prim_rec2_red T (FIX : forall o, F o (fun _ => T) -> T)
+        o (fx : F o Mu) :
+    prim_rec2 FIX (Con fx) = FIX _ (map (prim_rec2 FIX) fx).
   Proof.
     apply (prim_rec1_red FIX).
   Qed.
+
+
+
+(*
+
+  Definition rec_mem' (T : forall o, Mu o -> Type)
+             (FIX : forall o1 m1, 
+                 (forall o2 m2, mem m1 m2 -> T o2 m2) -> T o1 (Con' o1 m1)) :
+    forall o (m : Mu o), T o m.
+    apply rec. intros o1 m1 f.
+    destruct m1. apply FIX.
+    intros o2 m2 MEM. apply f, itn1_step, MEM.
+  Defined.
+
+  Lemma rec_mem'_red (T : forall o, Mu o -> Type)
+             (FIX : forall o1 m1, 
+                 (forall o2 m2, mem m1 m2 -> T o2 m2) -> T o1 (Con' o1 m1)) :
+    forall o m,
+      rec_mem' T FIX (Con' o m) = FIX _ m (fun o2 m2 _ => rec_mem' T FIX m2).
+  Proof.  
+    intros. apply iFix_eq.
+  Qed.
+
+  (* this is the most general one!! however i'm not sure it can be proven without K *)
+  Definition rec_mem2 (T : forall o, Mu o -> Type)
+             (FIX : forall o1 (m1 : F o1 Mu), 
+                 (forall o2 m2, mem m1 m2 -> T o2 m2) -> T o1 (Con m1)) :
+    forall o (m : Mu o), T o m.
+    apply rec_mem'.
+    intros. specialize (FIX _ (NTinv _ m1)).
+
+    unfold Con in FIX. rewrite BIJECTION2 in FIX. apply FIX.
+    intros. apply X0. apply MEM_COMMUTE in H0. rewrite BIJECTION2 in H0. apply H0.
+  Defined.
+
+  Lemma rec_mem_red2 (T : forall o, Mu o -> Type)
+        (FIX : forall o1 (m1 : F o1 Mu), 
+            (forall o2 (m2 : Mu o2), mem m1 m2 -> T o2 m2) -> T o1 (Con m1)) :
+    forall o (m : F o Mu),
+      rec_mem2 T FIX (Con m) = FIX _ m (fun o2 m2 _ => rec_mem2 T FIX m2).
+    intros. unfold Con. unfold rec_mem2 at 1. simpl.
+    rewrite rec_mem'_red. simpl.
+    
+    set (f := fun m' : F o Mu => (fun (o2 : O) (m2 : Mu o2) (_ : mem m' m2) => rec_mem2 T FIX m2)).
+
+    assert (eq_rect (NT Mu (NTinv Mu (NT Mu m)))
+    (fun c : Container P Mu =>
+     (forall (o2 : O) (m2 : Mu o2), mem (NTinv Mu (NT Mu m)) m2 -> T o2 m2) ->
+     T o (Con' o c)) (FIX o (NTinv Mu (NT Mu m))) (NT Mu m) 
+    (BIJECTION2 Mu (NT Mu m)) (f (NTinv Mu (NT Mu m))) =
+  FIX o m (f m)); [| apply H0].
+
+    simpl. remember (BIJECTION2 Mu (NT Mu m)). 
+  Admitted.
+
+  Lemma rec_mem_lemma o1 (m1 : Mu o1) o2 (m2 : Mu o2) :
+    mem (Des m1) m2 -> ord_c m2 m1.
+  Proof.
+    intro MEM. rewrite <- eta_expand2.
+    apply itn1_step, ord_correct, MEM.
+  Qed.
+
+  Definition rec_mem (T : forall o, Mu o -> Type)
+             (FIX : forall o1 (m1 : F o1 Mu), 
+                 (forall o2 (m2 : Mu o2), mem m1 m2 -> T o2 m2) -> T o1 (Con m1)) :
+    forall o (m : Mu o), T o m.
+    apply rec. intros o1 m1 f.
+
+    
+    rewrite <- eta_expand2. apply FIX. 
+
+    intros o2 m2 MEM. apply f. apply (rec_mem_lemma _ _ MEM).
+  Defined.
+
+  Lemma rec_mem_red (T : forall o, Mu o -> Type)
+        (FIX : forall o1 (m1 : F o1 Mu), 
+            (forall o2 (m2 : Mu o2), mem m1 m2 -> T o2 m2) -> T o1 (Con m1)) :
+    forall o (m : F o Mu),
+      rec_mem T FIX (Con m) = FIX _ m (fun o2 m2 _ => rec_mem T FIX m2).
+
+
+    intros. unfold rec_mem at 1. rewrite rec_red. simpl.
+    set (f := fun (m' : F o Mu) => fun (o2 : O) (m2 : Mu o2) (_ : mem m' m2) => rec_mem T FIX m2).
+    assert (eq_rect (Con (Des (Con m))) (T o)
+                    (FIX o (Des (Con m)) (f (Des (Con m)))) (Con m) (eta_expand2 (Con m)) =
+            FIX o m (f m)).
+    - remember (eta_expand2 (Con m)).
+
+      
+      assert (m' : Mu o). admit.
+      assert (Des m' = m). admit.
+      destruct H0. simpl. 
+
+      admit.
+
+  Definition Des2 : forall o, Mu o -> F o Mu :=
+    rec_mem (fun o _ => F o Mu) (fun _ m _ => m). 
+
+  Goal True. apply I. Qed.
+
+  Lemma Des2_eta1 : forall o (x : Mu o), Con (Des2 x) = x.
+  Proof.
+    apply rec_mem. intros o1 m1 FIX.
+    unfold Des2. rewrite rec_mem_red. reflexivity.
+  Qed.
+
+  Lemma Des2_eta2 : forall o (fx : F o Mu), Des2 (Con fx) = fx.
+  Proof.
+    intros. unfold Des2. rewrite rec_mem_red. reflexivity. 
+  Qed.
+*)
 
 End INDUCTIVE.
